autocommit 2018-03-25-12:00:12

framework/connectivity/ConnectedChecker2.v
@@ -229,7 +229,7 @@ Proof.
     apply IHcc.
 Qed.
 
-Definition max_aVarVset {a : A_set} (aVar : Var) (vT : V_set) : Prop :=
+Definition max_aVarVset (aVar : Var) (v : V_set) (a : A_set) (vT : V_set) : Prop :=
   (forall c1 c2 : Component, (vT c1 /\ a (A_ends c1 c2) /\ isa_aVarComponent aVar c2) -> vT c2).
 
 Lemma only_aVars_inaVarTree: forall (vT : V_set) (aT : A_set) (aVar : Var) (cc : aVarTree aVar vT aT) (x : Component),
@@ -371,7 +371,7 @@ Qed.
 
 Lemma aVarWalk_in_aVarTree: forall (aVar : Var) (vT : V_set) (aT : A_set) (cc : aVarTree aVar vT aT) 
                        (v1 v2: Component) (vl : V_list) (el : E_list) (w : Walk v a v1 v2 vl el),
-  max_aVarVset a aVar vT -> vT v1 -> aVarWalk aVar v1 v2 vl el w -> vT v2.
+  max_aVarVset aVar v a vT -> vT v1 -> aVarWalk aVar v1 v2 vl el w -> vT v2.
 Proof.
   intros aVar vT aT cc v1 v2 vl el w CC vTv1 aWalk.
   induction w ; unfold max_aVarVset in CC.
@@ -394,7 +394,7 @@ Qed.
 
 (* wenn sich zwei CCs in c \u00fcberschneiden, so sind \u00fcber c aVar-Walks m\u00f6glich und daher CC1 = CC2 *)
 Lemma two_aVarTrees_same_v: forall (aVar : Var) (v1 v2: V_set) (a1 a2: A_set) (c1 : aVarTree aVar v1 a1) (c2: aVarTree aVar v2 a2),
-  max_aVarVset aVar v1 -> max_aVarVset aVar v2 -> {c : Component & (v1 c /\ v2 c)} -> 
+  max_aVarVset aVar v a v1 -> max_aVarVset aVar v a v2 -> {c : Component & (v1 c /\ v2 c)} -> 
     (forall x : Component, v1 x -> v2 x).
 Proof.
   intros aVar v1 v2 a1 a2 c1 c2 acc1 acc2 same.
@@ -457,7 +457,7 @@ Proof.
 Qed.
 
 Lemma two_aVarTrees_same: forall (aVar : Var) (v1 v2: V_set) (a1 a2: A_set) (c1 : aVarTree aVar v1 a1) (c2: aVarTree aVar v2 a2),
-  max_aVarVset aVar v1 -> max_aVarVset aVar v2 -> {c : Component & (v1 c /\ v2 c)} -> 
+  max_aVarVset aVar v a v1 -> max_aVarVset aVar v a v2 -> {c : Component & (v1 c /\ v2 c)} -> 
     (v1 = v2).
 Proof.
   intros aVar v1 v2 a1 a2 c1 c2 acc1 acc2 same.
@@ -480,7 +480,7 @@ Proof.
 Qed.
 
 Lemma two_aVarTrees_same': forall (aVar : Var) (v1 v2: V_set) (a1 a2: A_set) (c1 : aVarTree aVar v1 a1) (c2: aVarTree aVar v2 a2),
-  max_aVarVset aVar v1 -> max_aVarVset aVar v2 -> {ar : Arc & (a1 ar /\ a2 ar)} -> 
+  max_aVarVset aVar v a v1 -> max_aVarVset aVar v a v2 -> {ar : Arc & (a1 ar /\ a2 ar)} -> 
     (v1 = v2).
 Proof.
   intros aVar v1 v2 a1 a2 c1 c2 acc1 acc2 same.
@@ -533,7 +533,7 @@ Definition root_of_Vset (vT : V_set) (root: Component) : Prop :=
   (vT root /\ forall (c : Component), vT c -> component_index c <= component_index root).
 
 Lemma root_same_aVarTrees_same : forall (aVar : Var) (vT1 vT2 : V_set) (aT1 aT2 : A_set),
-  aVarTree aVar vT1 aT1 -> aVarTree aVar vT2 aT2 -> max_aVarVset aVar vT1 -> max_aVarVset aVar vT2 ->
+  aVarTree aVar vT1 aT1 -> aVarTree aVar vT2 aT2 -> max_aVarVset aVar v a vT1 -> max_aVarVset aVar v a vT2 ->
   {c : Component & (root_of_Vset vT1 c /\ root_of_Vset vT2 c)} -> vT1 = vT2.
 Proof.
   intros aVar vT1 vT2 aT1 aT2 aTree1 aTree2 maTree1 maTree2 H.
@@ -621,7 +621,7 @@ Proof.
 Qed.
 
 Lemma aVarTrees_same_root_same : forall (aVar : Var) (vT1 vT2 : V_set) (aT1 aT2 : A_set),
-  aVarTree aVar vT1 aT1 -> aVarTree aVar vT2 aT2 -> max_aVarVset a aVar vT1 -> max_aVarVset aVar vT2 ->
+  aVarTree aVar vT1 aT1 -> aVarTree aVar vT2 aT2 -> max_aVarVset aVar v a vT1 -> max_aVarVset aVar v a vT2 ->
   vT1 = vT2 -> {c : Component & (root_of_Vset vT1 c /\ root_of_Vset vT2 c)}.
 Proof.
   intros aVar vT1 vT2 aT1 aT2 aTree1 aTree2 maTree1 maTree2 vT1vT2.
@@ -641,52 +641,36 @@ Qed.
 Definition is_aVarspanning (aVar : Var) (vT : V_set) : Prop := 
   forall c, (v c /\ isa_aVarComponent aVar c) -> vT c.
 
-Definition all_aVarTreesSame (aVar : Var) : Prop :=
+Definition all_maxaVarTreesSame (aVar : Var) (v : V_set) (a : A_set) : Prop :=
 (forall vT1 vT2 aT1 aT2 (aTree1 : aVarTree aVar vT1 aT1) (aTree2 : aVarTree aVar vT2 aT2),
-    (max_aVarVset aVar vT1 /\ max_aVarVset aVar vT2) ->
+    (max_aVarVset aVar v a vT1 /\ max_aVarVset aVar v a vT2) ->
     vT1 = vT2).
 
-Lemma aVarTree_maxTree : forall (aVar : Var) (vT : V_set) (aT : A_set),
-  aVarTree aVar vT aT -> 
-  {vT2 : V_set & {aT2 : A_set & {maTree : aVarTree aVar vT2 aT2 & 
-    (max_aVarVset aVar vT2 /\ V_included vT vT2 /\ A_included aT aT2)}}}.
+Lemma one_arc_doesnt_matter_allSame : forall (aVar : Var) (v : V_set) (a : A_set) (g : Connected v a) (x y : Component),
+  all_maxaVarTreesSame aVar v (A_union (E_set x y) a) ->  all_maxaVarTreesSame aVar v a.
+Proof.
+Admitted.
+
+Lemma one_arc_doesnt_matter_aVarVset : 
+  forall (aVar : Var) (v : V_set) (a : A_set) (vT : V_set) (aT : A_set) (x y : Component),
+  aVarTree aVar vT aT -> max_aVarVset aVar v a vT -> all_maxaVarTreesSame aVar v a ->
+  max_aVarVset aVar v (A_union (E_set x y) a) vT.
 Proof.
   intros.
 Admitted.
 
 Lemma allMaxTreesSame_spanningTree : forall (aVar : Var) (vT : V_set) (aT : A_set),
-   all_aVarTreesSame aVar -> aVarTree aVar vT aT -> max_aVarVset aVar vT -> 
+   all_maxaVarTreesSame aVar v a -> aVarTree aVar vT aT -> max_aVarVset aVar v a vT -> 
   is_aVarspanning aVar vT.
 Proof.
   intros aVar vT aT allSame aTree maTree.
-(*   assert ({v0 : V_set & {a0 : A_set & Connected v0 a0}}).
-  exists v.
-  exists a.
-  apply g.
-  destruct X.
-  destruct s.
- *)  induction g. unfold is_aVarspanning in * ; unfold all_aVarTreesSame in * ; intros.
-  + clear x.
-    assert (aVarTree aVar (V_single c) A_empty).
+  induction g. unfold is_aVarspanning in * ; unfold all_maxaVarTreesSame in * ; intros.
+  + assert (aVarTree aVar (V_single c) A_empty).
     destruct H.
     apply CC_isolated.
     auto.
     auto.
-(*     (* *)apply (aVarTree_maxTree) in H0.
-    destruct H0.
-    destruct s.
-    destruct s.
-    destruct a0.
-    destruct H1.
-    specialize (allSame vT x aT x0 aTree x1).
-    assert (vT = x).
-    auto.
-    unfold V_included in H1.
-    unfold Included in H1.
-    rewrite H3.
-    apply (H1 c).
-    apply In_single.    *) 
-(* *)specialize (allSame vT (V_single c) aT A_empty aTree H0).
+    specialize (allSame vT (V_single c) aT A_empty aTree H0).
     assert (vT = V_single c).
     apply allSame.
     split.
@@ -695,35 +679,17 @@ Proof.
     intros.
     destruct H1.
     destruct H2.
-    assert (a = A_empty).
-    admit.
-    rewrite H4 in *.
     inversion H2.
-    assert (vT = V_single c).
-    apply allSame.
-    auto.
-    rewrite H2.
+    rewrite H1.
     apply In_single.
-
-(* (* *)specialize (allSame vT (V_single c) aT A_empty aTree H0).
-    assert (max_aVarVset aVar (V_single c)).
-    unfold max_aVarVset.
-    intros.
-    destruct H1.
-    destruct H2.
-    assert (a = A_empty).
+  + (* apply IHc.
+    unfold all_maxaVarTreesSame in *.
+    intros. *)
     admit.
-    rewrite H4 in *.
-    inversion H2.
-    assert (vT = V_single c).
-    apply allSame.
+  + apply IHc ; clear IHc.
+    apply (one_arc_doesnt_matter_allSame aVar v0 a0 c x y).
     auto.
-    rewrite H2.
-    apply In_single.
- *)  + apply (IHc c0).
-    apply H.
-  + apply (IHc c0).
-    apply H.
+    apply (one_arc_doesnt_matter_aVarVset aVar v0 a0 
   + apply (IHc c0).
     apply H.
 Qed.
